src/Database/Manifest.v
@@ -7,12 +7,10 @@ From RecoveryRefinement Require Import Database.Table.
 
 Module Manifest.
   Module Mft.
-    (* TODO: would be good to have arrays of tables, but tables are not
-    represented by a type code (they're records) *)
     Record t :=
-      mk { l0tables: list Table.Tbl.t;
-           l1tables: list Table.Tbl.t;
-           nextIdent: IORef ty.uint32;
+      mk { l0tables: Array Table.Tbl.t;
+           l1tables: Array Table.Tbl.t;
+           nextIdent: IORef uint32;
          }.
   End Mft.
 End Manifest.
